Refactor ConstrainedAction
Signed-off-by: zeramorphic <zeramorphic@proton.me>

ConNF/Foa/Properties/ConstrainedAction.lean
@@ -10,14 +10,14 @@ namespace ConNF
 
 namespace StructApprox
 
-variable [Params.{u}] {α : Λ} [BasePositions] [FoaAssumptions α] {β : Iic α}
+variable [Params.{u}] [BasePositions] [Level] [FoaAssumptions] {β : Λ} [LeLevel β]
   [FreedomOfActionHypothesis β]
 
 def transConstrained (c d : SupportCondition β) : Set (SupportCondition β) :=
-  {e | e <[α] c} ∪ {e | e <[α] d}
+  {e | e < c} ∪ {e | e < d}
 
 def reflTransConstrained (c d : SupportCondition β) : Set (SupportCondition β) :=
-  {e | e ≤[α] c} ∪ {e | e ≤[α] d}
+  {e | e ≤ c} ∪ {e | e ≤ d}
 
 theorem transConstrained_symm (c d : SupportCondition β) :
     transConstrained c d = transConstrained d c :=
@@ -28,12 +28,12 @@ theorem reflTransConstrained_symm (c d : SupportCondition β) :
   union_comm _ _
 
 @[simp]
-theorem transConstrained_self (c : SupportCondition β) : transConstrained c c = {e | e <[α] c} :=
+theorem transConstrained_self (c : SupportCondition β) : transConstrained c c = {e | e < c} :=
   union_self _
 
 @[simp]
 theorem reflTransConstrained_self (c : SupportCondition β) :
-    reflTransConstrained c c = {e | e ≤[α] c} :=
+    reflTransConstrained c c = {e | e ≤ c} :=
   union_self _
 
 theorem mem_reflTransConstrained_of_mem_transConstrained {c d e : SupportCondition β}
@@ -43,19 +43,19 @@ theorem mem_reflTransConstrained_of_mem_transConstrained {c d e : SupportConditi
   exact Or.inr he.to_reflTransGen
 
 theorem transConstrained_trans {c d e f : SupportCondition β} (he : e ∈ transConstrained c d)
-    (hf : f ≤[α] e) : f ∈ transConstrained c d := by
+    (hf : f ≤ e) : f ∈ transConstrained c d := by
   obtain he | he := he
   exact Or.inl (Relation.TransGen.trans_right hf he)
   exact Or.inr (Relation.TransGen.trans_right hf he)
 
 theorem reflTransConstrained_trans {c d e f : SupportCondition β}
-    (he : e ∈ reflTransConstrained c d) (hf : f ≤[α] e) : f ∈ reflTransConstrained c d := by
+    (he : e ∈ reflTransConstrained c d) (hf : f ≤ e) : f ∈ reflTransConstrained c d := by
   obtain he | he := he
   exact Or.inl (hf.trans he)
   exact Or.inr (hf.trans he)
 
 theorem transConstrained_of_reflTransConstrained_of_trans_constrains {c d e f : SupportCondition β}
-    (he : e ∈ reflTransConstrained c d) (hf : f <[α] e) : f ∈ transConstrained c d := by
+    (he : e ∈ reflTransConstrained c d) (hf : f < e) : f ∈ transConstrained c d := by
   obtain he | he := he
   exact Or.inl (hf.trans_left he)
   exact Or.inr (hf.trans_left he)
@@ -86,8 +86,8 @@ theorem fst_mem_transConstrained {c d : SupportCondition β} {A : ExtendedIndex 
     (hN : ⟨A, inr N⟩ ∈ transConstrained c d) :
     ⟨A, inr N.fst.toNearLitter⟩ ∈ transConstrained c d := by
   obtain hN | hN := hN
-  exact Or.inl (transConstrains_nearLitter' hN)
-  exact Or.inr (transConstrains_nearLitter' hN)
+  exact Or.inl (lt_nearLitter' hN)
+  exact Or.inr (lt_nearLitter' hN)
 
 theorem fst_mem_refl_trans_constrained' {c d : SupportCondition β} {A : ExtendedIndex β} {a : Atom}
     (h : ⟨A, inl a⟩ ∈ reflTransConstrained c d) :
@@ -98,8 +98,8 @@ theorem fst_mem_reflTransConstrained {c d : SupportCondition β} {A : ExtendedIn
     {N : NearLitter} (hN : ⟨A, inr N⟩ ∈ reflTransConstrained c d) :
     ⟨A, inr N.fst.toNearLitter⟩ ∈ reflTransConstrained c d := by
   obtain hN | hN := hN
-  exact Or.inl (reflTransConstrains_nearLitter hN)
-  exact Or.inr (reflTransConstrains_nearLitter hN)
+  exact Or.inl (le_nearLitter hN)
+  exact Or.inr (le_nearLitter hN)
 
 theorem fst_mem_transConstrained_of_mem_symmDiff {c d : SupportCondition β} {A : ExtendedIndex β}
     {N : NearLitter} {a : Atom} (h : a ∈ litterSet N.1 ∆ N)
@@ -149,22 +149,22 @@ theorem eq_of_sublitter_bijection_apply_eq {π : NearLitterApprox} {L₁ L₂ L�
 noncomputable def constrainedAction (π : StructApprox β) (s : Set (SupportCondition β))
     (hs : Small s) : StructAction β := fun B =>
   { atomMap := fun a =>
-      ⟨∃ c : SupportCondition β, c ∈ s ∧ ⟨B, inl a⟩ ≤[α] c,
+      ⟨∃ c : SupportCondition β, c ∈ s ∧ ⟨B, inl a⟩ ≤ c,
         fun _ => π.completeAtomMap B a⟩
     litterMap := fun L =>
-      ⟨∃ c : SupportCondition β, c ∈ s ∧ ⟨B, inr L.toNearLitter⟩ ≤[α] c,
+      ⟨∃ c : SupportCondition β, c ∈ s ∧ ⟨B, inr L.toNearLitter⟩ ≤ c,
         fun _ => π.completeNearLitterMap B L.toNearLitter⟩
     atomMap_dom_small := by
       change Small ((fun a : Atom => ⟨B, inl a⟩) ⁻¹'
-        {c : SupportCondition β | ∃ d : SupportCondition β, d ∈ s ∧ c ≤[α] d})
-      refine' Small.preimage _ (reflTransClosure_small α hs)
+        {c : SupportCondition β | ∃ d : SupportCondition β, d ∈ s ∧ c ≤ d})
+      refine' Small.preimage _ (reflTransClosure_small hs)
       intro a b h
       cases h
       rfl
     litterMap_dom_small := by
       change Small ((fun L : Litter => ⟨B, inr L.toNearLitter⟩) ⁻¹'
-        {c : SupportCondition β | ∃ d : SupportCondition β, d ∈ s ∧ c ≤[α] d})
-      refine' Small.preimage _ (reflTransClosure_small α hs)
+        {c : SupportCondition β | ∃ d : SupportCondition β, d ∈ s ∧ c ≤ d})
+      refine' Small.preimage _ (reflTransClosure_small hs)
       intro a b h
       cases h
       rfl }
@@ -188,7 +188,7 @@ noncomputable def ihsAction (π : StructApprox β) (c d : SupportCondition β) :
 theorem constrainedAction_atomMap {π : StructApprox β} {s : Set (SupportCondition β)} {hs : Small s}
     {B : ExtendedIndex β} {a : Atom} :
     (constrainedAction π s hs B).atomMap a =
-      ⟨∃ c : SupportCondition β, c ∈ s ∧ ⟨B, inl a⟩ ≤[α] c,
+      ⟨∃ c : SupportCondition β, c ∈ s ∧ ⟨B, inl a⟩ ≤ c,
         fun _ => completeAtomMap π B a⟩ :=
   rfl
 
@@ -196,7 +196,7 @@ theorem constrainedAction_atomMap {π : StructApprox β} {s : Set (SupportCondit
 theorem constrainedAction_litterMap {π : StructApprox β} {s : Set (SupportCondition β)}
     {hs : Small s} {B : ExtendedIndex β} {L : Litter} :
     (constrainedAction π s hs B).litterMap L =
-      ⟨∃ c : SupportCondition β, c ∈ s ∧ ⟨B, inr L.toNearLitter⟩ ≤[α] c,
+      ⟨∃ c : SupportCondition β, c ∈ s ∧ ⟨B, inr L.toNearLitter⟩ ≤ c,
         fun _ => π.completeNearLitterMap B L.toNearLitter⟩ :=
   rfl
 
@@ -244,7 +244,7 @@ theorem constrainedAction_mono {π : StructApprox β} {s t : Set (SupportConditi
     ⟨fun _ hL => ⟨hL.choose, h hL.choose_spec.1, hL.choose_spec.2⟩, fun _ _ => rfl⟩⟩
 
 theorem ihAction_le_constrainedAction {π : StructApprox β} {s : Set (SupportCondition β)}
-    {hs : Small s} (c : SupportCondition β) (hc : ∃ d : SupportCondition β, d ∈ s ∧ c ≤[α] d) :
+    {hs : Small s} (c : SupportCondition β) (hc : ∃ d : SupportCondition β, d ∈ s ∧ c ≤ d) :
     ihAction (π.foaHypothesis : HypAction c) ≤ constrainedAction π s hs :=
   fun _ =>
   ⟨⟨fun _ ha => ⟨hc.choose, hc.choose_spec.1, _root_.trans ha.to_reflTransGen hc.choose_spec.2⟩,
@@ -259,16 +259,16 @@ theorem ihAction_eq_constrainedAction (π : StructApprox β) (c : SupportConditi
   ext
   · funext
     ext
-    simp only [ihAction_atomMap, foaHypothesis_atomImage, Part.mem_mk_iff,
-      Relation.TransGen.tail'_iff, exists_prop,
-      constrainedAction_atomMap, mem_setOf_eq, and_congr_left_iff]
+    simp only [ihAction_atomMap, foaHypothesis_atomImage, Part.mem_mk_iff, SupportCondition.lt_iff,
+      Relation.TransGen.tail'_iff, exists_prop, constrainedAction_atomMap, mem_setOf_eq,
+      SupportCondition.le_iff, and_congr_left_iff]
     intro
     simp_rw [and_comm]
   · funext
     ext
     simp only [ihAction_litterMap, foaHypothesis_nearLitterImage, Part.mem_mk_iff,
-      Relation.TransGen.tail'_iff, exists_prop,
-      constrainedAction_litterMap, mem_setOf_eq, and_congr_left_iff]
+      SupportCondition.lt_iff, Relation.TransGen.tail'_iff, exists_prop,
+      constrainedAction_litterMap, mem_setOf_eq, SupportCondition.le_iff, and_congr_left_iff]
     intro
     simp_rw [and_comm]
 
@@ -280,9 +280,10 @@ theorem ihsAction_eq_constrainedAction (π : StructApprox β) (c d : SupportCond
   ext
   · funext
     ext
-    simp only [Relation.TransGen.tail'_iff, transConstrained, mem_union, ihsAction_atomMap,
-      Part.mem_mk_iff, exists_prop, mem_setOf_eq, constrainedAction_atomMap, and_congr_left_iff]
-    intro
+    simp only [ihsAction_atomMap, transConstrained, Part.mem_mk_iff, mem_union, mem_setOf_eq,
+      exists_prop, constrainedAction_atomMap, and_congr_left_iff]
+    simp only [SupportCondition.lt_iff, SupportCondition.le_iff, Relation.TransGen.tail'_iff]
+    rintro rfl
     constructor
     · rintro (⟨b, hb₁, hb₂⟩ | ⟨b, hb₁, hb₂⟩)
       · exact ⟨b, Or.inl hb₂, hb₁⟩
@@ -292,9 +293,9 @@ theorem ihsAction_eq_constrainedAction (π : StructApprox β) (c d : SupportCond
       · exact Or.inr ⟨b, hb₂, hb₁⟩
   · funext
     ext
-    simp only [Relation.TransGen.tail'_iff, transConstrained, mem_union, Part.mem_mk_iff,
-      exists_prop, mem_setOf_eq, and_congr_left_iff, ihsAction_litterMap,
-      constrainedAction_litterMap]
+    simp only [ihsAction_litterMap, transConstrained, Part.mem_mk_iff, mem_union, mem_setOf_eq,
+      exists_prop, constrainedAction_litterMap, and_congr_left_iff]
+    simp only [SupportCondition.lt_iff, SupportCondition.le_iff, Relation.TransGen.tail'_iff]
     intro
     constructor
     · rintro (⟨b, hb₁, hb₂⟩ | ⟨b, hb₁, hb₂⟩)
@@ -308,7 +309,7 @@ theorem ihAction_le_ihsAction (π : StructApprox β) (c d : SupportCondition β)
     ihAction (π.foaHypothesis : HypAction c) ≤ ihsAction π c d :=
   fun _ => ⟨⟨fun _ => Or.inl, fun _ _ => rfl⟩, ⟨fun _ => Or.inl, fun _ _ => rfl⟩⟩
 
-theorem ihAction_le {π : StructApprox β} {c d : SupportCondition β} (h : c ≤[α] d) :
+theorem ihAction_le {π : StructApprox β} {c d : SupportCondition β} (h : c ≤ d) :
     ihAction (π.foaHypothesis : HypAction c) ≤ ihAction (π.foaHypothesis : HypAction d) := by
   refine' fun B => ⟨⟨_, fun a h => rfl⟩, ⟨_, fun L h => rfl⟩⟩
   · intro a ha
@@ -317,17 +318,18 @@ theorem ihAction_le {π : StructApprox β} {c d : SupportCondition β} (h : c �
     exact Relation.TransGen.trans_left ha h
 
 theorem transGen_constrains_of_mem_designatedSupport {A : ExtendedIndex β} {L : Litter}
-    {h : InflexibleCoe A L} {γ : Iic α} {δ ε : Iio α} {hδ : (δ : Λ) < γ} {hε : (ε : Λ) < γ}
-    (hδε : δ ≠ ε) {C : Path (h.path.δ : TypeIndex) γ} {t : Tangle δ}
+    {h : InflexibleCoe A L} {γ δ ε : Iio α} [LeLevel γ] [LtLevel δ] [LtLevel ε]
+    {hδ : (δ : TypeIndex) < γ} {hε : (ε : TypeIndex) < γ}
+    (hδε : (δ : TypeIndex) ≠ ε) {C : Path (h.path.δ : TypeIndex) γ} {t : Tangle δ}
     {d : SupportCondition h.path.δ}
-    (hd₂ : ⟨(C.cons (coe_lt hε)).cons (bot_lt_coe _),
-      inr (fuzz (Subtype.coe_injective.ne (Iio.coe_injective.ne hδε)) t).toNearLitter⟩ ≤[α] d)
-    (hd : ⟨(h.path.B.cons (coe_lt h.path.hδ)).comp d.path, d.value⟩ ≺ ⟨A, inr L.toNearLitter⟩)
+    (hd₂ : ⟨(C.cons hε).cons (bot_lt_coe _),
+      inr (fuzz hδε t).toNearLitter⟩ ≤ d)
+    (hd : ⟨(h.path.B.cons h.path.hδ).comp d.path, d.value⟩ ≺ ⟨A, inr L.toNearLitter⟩)
     {B : ExtendedIndex δ} {a : Atom} (hc : ⟨B, inl a⟩ ∈ (designatedSupport t).carrier) :
-    ⟨(h.path.B.cons (coe_lt h.path.hδ)).comp ((C.cons (coe_lt hδ)).comp B), inl a⟩ <[α]
+    (⟨(h.path.B.cons h.path.hδ).comp ((C.cons hδ).comp B), inl a⟩ : SupportCondition β) <
       ⟨A, inr L.toNearLitter⟩ := by
   refine' Relation.TransGen.tail' _ hd
-  refine' reflTransConstrains_comp (c := ⟨_, inl a⟩) (d := d) _ (h.path.B.cons <| coe_lt h.path.hδ)
+  refine' le_comp (c := ⟨_, inl a⟩) _ (h.path.B.cons h.path.hδ)
   refine' Relation.ReflTransGen.trans _ hd₂
   exact Relation.ReflTransGen.single (Constrains.fuzz hδ hε hδε C t _ hc)
 
